changes to tactic

src/ecAst.mli
@@ -165,9 +165,7 @@ and mty_mr = module_type * mod_restr
 and mty_mr_qb = mty_mr * qbounds 
 
 and qbounds = (xpath * int) list
-and qmod_or_proc =
-  | Qmod of EcPath.mpath
-  | Qproc of EcPath.xpath
+
 
 and binding  = (EcIdent.t * gty)
 and bindings = binding list
@@ -322,7 +320,7 @@ and pr = {
 }
 
 and qbound = {
-  qb_proc : qmod_or_proc;
+  qb_proc : xpath;
   qb_orcl : xpath;
   qb_bound : form;
 }
@@ -563,8 +561,6 @@ val eg_hash   : eagerF hash
 
 val pr_equal  : pr equality
 val pr_hash   : pr hash
-
-val qmod_or_proc_equal : qmod_or_proc equality
 
 val qb_equal  : qbound equality
 val qb_hash   : qbound hash
