src/ecFol.mli
@@ -263,6 +263,6 @@ end
 (* -------------------------------------------------------------------- *)
 val dump_f : form -> string
 
-val proc_of_qbound : form -> qmod_or_proc
+val proc_of_qbound : form -> xpath
 val orcl_of_qbound : form -> xpath
 val bound_of_qbound : form -> form
