src/phl/ecPhlQbound.ml
@@ -13,15 +13,41 @@ let c    = f_local c_id EcTypes.tint
 
 let check (a : EcDecl.axiom) (callee : xpath) (f : xpath) (o : xpath) (env : env) : bool =
   let form = a.ax_spec in
-  match form.f_node with 
-  | Fqbound qb -> 
-    (*Format.eprintf "f'1 = %s\n%!" (EcFol.dump_f form);*)
+  match form.f_node with
+  | Fqbound qb ->(*
+    begin 
+      Format.eprintf "[qbound-check] qb.proc=%s qb.orcl=%s qb.bound=%s@."
+        (EcPath.x_tostring qb.qb_proc)
+        (EcPath.x_tostring qb.qb_orcl)
+        (EcFol.dump_f qb.qb_bound);
+      Format.eprintf "[qbound-check] callee=%s@." (EcPath.x_tostring callee);
+      Format.eprintf "[qbound-check] f=%s@." (EcPath.x_tostring f);
+
+      let sin1 = NormMp.sig_of_mp env callee.x_top in
+      let sin2 = NormMp.sig_of_mp env f.x_top in
+      let me1, _ = Mod.by_mpath qb.qb_proc.x_top env in
+      let me2, _ = Mod.by_mpath qb.qb_orcl.x_top env in
+      let mt1, mt2 =
+        match me1.me_body, me2.me_body with
+        | ME_Decl mty1, ME_Decl mty2 -> mty1, mty2
+        | _ -> assert false
+      in
+
+      (* Match both module type and called procedure/oracle symbols. *)
+      try
+        EcTyping.check_modtype env callee.x_top sin1 mt1;
+        EcTyping.check_modtype env f.x_top sin2 mt2;
+        EcSymbols.sym_equal callee.x_sub qb.qb_proc.x_sub
+        && EcSymbols.sym_equal f.x_sub qb.qb_orcl.x_sub
+      with
+      | _ -> false
+    end *)
     let s = f_bind_mod (f_subst_init ()) (mget_ident qb.qb_orcl.x_top) f.x_top env in
     let f' = EcCoreSubst.Fsubst.f_subst s form in
     (*Format.eprintf "f'2 = %s\n%!" (EcFol.dump_f f');*)
     begin
     match f'.f_node with     
-      |Fqbound qb -> (*qmod_or_proc_equal qb.qb_proc (Qproc callee) &&*) x_equal qb.qb_orcl o
+      |Fqbound qb -> (*qmod_or_proc_equal qb.qb_proc (Qproc callee) &&*) x_equal qb.qb_orcl o && EcSymbols.sym_equal callee.x_sub qb.qb_proc.x_sub
       | _ -> assert false
     end
   | _ -> false
@@ -34,6 +60,9 @@ let rec qbound_concrete (fb : stmt) (o : xpath) (env : env) =
   let doit i =
     match i.i_node with
     | Scall (_, x, _) -> 
+
+       let x = NormMp.norm_xfun env x in
+       Format.eprintf "[debug] xpath x: %s\n%!" (EcPath.x_tostring x);
        let f' = Fun.by_xpath x env in
        begin
        let cmag = if f'.f_quantum = `Quantum then c else f_i1 in
@@ -51,10 +80,13 @@ let rec qbound_concrete (fb : stmt) (o : xpath) (env : env) =
 
 and qbound_abstract (callee : xpath) (ois : oracle_info) (o : xpath) (env : env) =
   let ois = List.map (NormMp.norm_xfun env) ois.oi_calls in
-  (*List.iter (fun x -> Format.eprintf "oracle : %s\n%!" (EcPath.x_tostring x)) ois;*)
-  if not (List.exists (fun o' -> x_equal o o') ois) then f_i0
+  List.iter (fun x -> Format.eprintf "oracle : %s\n%!" (EcPath.x_tostring x)) ois;
+  if not (List.exists (fun o' -> x_equal o o') ois) then (Format.eprintf "no oracle calls to: %s\n%!" (EcPath.x_tostring o); f_i0)
   else
   let doit oi =
+    
+    let oi = NormMp.norm_xfun env oi in
+    Format.eprintf "[debug] xpath oi: %s\n%!" (EcPath.x_tostring oi);
     let f = Fun.by_xpath oi env in
     (*Format.eprintf "quantum : %a\n%!" EcPrinting.pp_quantum f.f_quantum;*)
     let cmag = if f.f_quantum = `Quantum then c else f_i1 in
@@ -71,7 +103,7 @@ and qbound_abstract (callee : xpath) (ois : oracle_info) (o : xpath) (env : env)
     match (List.hd l).ax_spec.f_node with Fqbound qb -> f_int_mul qb.qb_bound qo | _ -> assert false
   in
   let l = List.snd (Ax.all ~check:(fun _ a -> List.exists (fun o' -> check a callee o' o env) ois) env) in
-  if List.is_empty l then f_i0
+  if List.is_empty l then (Format.eprintf "Check \n%!"; f_i0)
   else
   let qb = match (List.hd l).ax_spec.f_node with Fqbound qb -> qb .qb_bound| _ -> assert false in
   sum_int_forms (List.map doit ois) |> f_int_add_simpl qb
@@ -83,9 +115,6 @@ let process_qbound (tc : tcenv1) =
   let env = FApi.tc1_env tc in
   let x = proc_of_qbound q in
   let o = orcl_of_qbound q in
-  let x = match x with 
-    | Qproc p -> p
-    | Qmod _ -> assert false in
   let f = Fun.by_xpath x env in
   let sum = match f.f_def with | FBdef fb -> qbound_concrete fb.f_body o env | _ -> assert false in
   FApi.xmutate1 tc `Qbound [f_int_le qb sum]
